

# Problem 12.529

Sujal Rajani

October 12, 2025

## Question

### Question:

Let  $\mathbf{M}$  be a  $3 \times 3$  matrix and suppose that 1, 2 and 3 are the eigenvalues of  $\mathbf{M}$ . If

$$\mathbf{M}^{-1} = \frac{\mathbf{M}^2 - \mathbf{M} + \mathbf{I}_3}{\alpha} \quad (1.1)$$

for some scalar  $\alpha \neq 0$ , then  $\alpha$  is equal to \_\_\_\_.

## Solution

**SOLUTION Solution:**

**Solution:**

Let  $\lambda$  be an eigenvalue of  $\mathbf{M}$ , and  $\mathbf{v}$  the corresponding eigenvector:

$$\mathbf{M}\mathbf{v} = \lambda\mathbf{v} \quad (1.2)$$

Applying both sides to the given identity:

$$\mathbf{M}^{-1}\mathbf{v} = \frac{\mathbf{M}^2 - \mathbf{M} + \mathbf{I}_3}{\alpha}\mathbf{v} \quad (1.3)$$

## Step-by-Step Calculation

Since polynomial expressions in  $\mathbf{M}$  act on eigenvectors by substituting  $\lambda$  for  $\mathbf{M}$ , we have:

$$\mathbf{M}^2 \mathbf{v} = \lambda^2 \mathbf{v}, \quad \mathbf{I}_3 \mathbf{v} = \mathbf{v} \quad (1.4)$$

Thus,

$$\mathbf{M}^{-1} \mathbf{v} = \frac{\lambda^2 - \lambda + 1}{\alpha} \mathbf{v} \quad (1.5)$$

But

$$\mathbf{M}^{-1} \mathbf{v} = \frac{1}{\lambda} \mathbf{v} \quad (1.6)$$

Therefore,

$$\frac{1}{\lambda} = \frac{\lambda^2 - \lambda + 1}{\alpha} \implies \alpha = \lambda(\lambda^2 - \lambda + 1) \quad (1.7)$$

## Frame Title

For the three eigenvalues, compute  $\alpha$ :

For  $\lambda = 1$ :

$$\alpha = 1 \times (1^2 - 1 + 1) = 1 \quad (1.8)$$

For  $\lambda = 2$ :

$$\alpha = 2 \times (2^2 - 2 + 1) = 2 \times (4 - 2 + 1) = 6 \quad (1.9)$$

For  $\lambda = 3$ :

$$\alpha = 3 \times (9 - 3 + 1) = 3 \times 7 = 21 \quad (1.10)$$

Thus, there is no single  $\alpha$  that satisfies all three cases, so the expression does not hold for all eigenvalues simultaneously.